Give more canonical names to some theorems

PossiblyInfiniteTrees/PossiblyInfiniteTree/PossiblyInfiniteTree.lean
@@ -2,10 +2,15 @@ import PossiblyInfiniteTrees.PossiblyInfiniteTree.InfiniteTree
 
 structure PossiblyInfiniteTree (α : Type u) where
   infinite_tree : InfiniteTreeSkeleton (Option α)
-  no_orphans : ∀ node : List Nat, infinite_tree node ≠ none -> ∀ parent : { l : List Nat // ∃ diff, diff ++ l = node }, infinite_tree parent ≠ none
-  no_holes_in_children : ∀ node : List Nat, ∀ n : Nat, (infinite_tree.children node) n ≠ none -> ∀ m : Fin n, (infinite_tree.children node) m ≠ none
+  no_orphans : 
+    ∀ node : List Nat, infinite_tree node ≠ none -> 
+    ∀ parent : { l : List Nat // ∃ diff, diff ++ l = node }, infinite_tree parent ≠ none
+  no_holes_in_children :
+    ∀ node : List Nat, ∀ n : Nat, (infinite_tree.children node) n ≠ none -> 
+    ∀ m : Fin n, (infinite_tree.children node) m ≠ none
 
 namespace PossiblyInfiniteTree
+
   def get (tree : PossiblyInfiniteTree α) (node : List Nat) : Option α := tree.infinite_tree node
 
   def children (tree : PossiblyInfiniteTree α) (node : List Nat) : PossiblyInfiniteList α := {
@@ -13,7 +18,7 @@ namespace PossiblyInfiniteTree
     no_holes := by apply tree.no_holes_in_children
   }
 
-  theorem children_empty_when_not_existing (tree : PossiblyInfiniteTree α) (node : List Nat) : tree.get node = none -> tree.children node = PossiblyInfiniteList.empty := by
+  theorem children_empty_of_get_eq_none (tree : PossiblyInfiniteTree α) (node : List Nat) : tree.get node = none -> tree.children node = PossiblyInfiniteList.empty := by
     intro h
     unfold children
     unfold PossiblyInfiniteList.empty
@@ -30,7 +35,7 @@ namespace PossiblyInfiniteTree
       exact contra
     contradiction
 
-  theorem children_empty_means_all_following_none (tree : PossiblyInfiniteTree α) (node : List Nat) : tree.children node = PossiblyInfiniteList.empty -> ∀ i, tree.get (i :: node) = none := by
+  theorem each_successor_none_of_children_empty (tree : PossiblyInfiniteTree α) (node : List Nat) : tree.children node = PossiblyInfiniteList.empty -> ∀ i, tree.get (i :: node) = none := by
     intro h i
     unfold get
     unfold children at h
@@ -40,7 +45,7 @@ namespace PossiblyInfiniteTree
     apply congr h
     rfl
 
-  theorem first_child_none_means_children_empty (tree : PossiblyInfiniteTree α) (node : List Nat) : tree.get (0::node) = none -> tree.children node = PossiblyInfiniteList.empty := by
+  theorem children_empty_of_first_successor_none (tree : PossiblyInfiniteTree α) (node : List Nat) : tree.get (0::node) = none -> tree.children node = PossiblyInfiniteList.empty := by
     intro h
     unfold PossiblyInfiniteList.empty
     unfold children
@@ -59,7 +64,7 @@ namespace PossiblyInfiniteTree
       specialize no_holes contra ⟨0, by simp⟩
       contradiction
 
-  theorem getElem_children_eq_get_tree (tree : PossiblyInfiniteTree α) (node : List Nat) (index : Nat) : (tree.children node).infinite_list index = tree.get (index :: node) := by
+  theorem getElem_children_eq_get (tree : PossiblyInfiniteTree α) (node : List Nat) (index : Nat) : (tree.children node).infinite_list index = tree.get (index :: node) := by
     unfold children
     unfold get
     unfold InfiniteTreeSkeleton.children
@@ -71,12 +76,12 @@ namespace PossiblyInfiniteTree
   def branches (tree : PossiblyInfiniteTree α) : Set (PossiblyInfiniteList α) := fun pil =>
     pil.infinite_list ∈ tree.infinite_tree.branches
 
-  theorem branches_through_eq_union_children (tree : PossiblyInfiniteTree α) (node : List Nat) : tree.branches_through node = fun b => ∃ (i : Nat), b ∈ tree.branches_through (i :: node) := by
+  theorem branches_through_eq_union_branches_through_successors (tree : PossiblyInfiniteTree α) (node : List Nat) : tree.branches_through node = fun b => ∃ (i : Nat), b ∈ tree.branches_through (i :: node) := by
     unfold branches_through
     apply funext
     simp
     intro pil
-    rw [tree.infinite_tree.branches_through_eq_union_children]
+    rw [tree.infinite_tree.branches_through_eq_union_branches_through_successors]
     constructor
     . intro h
       rcases h with ⟨i, h⟩
@@ -86,5 +91,6 @@ namespace PossiblyInfiniteTree
       exists i
 
   def leaves (tree : PossiblyInfiniteTree α) : Set α := fun a => ∃ node : List Nat, tree.get node = some a ∧ tree.children node = PossiblyInfiniteList.empty
+
 end PossiblyInfiniteTree
 
