PossiblyInfiniteTrees/PossiblyInfiniteTree/InfiniteTree.lean
@@ -15,10 +15,10 @@ namespace InfiniteTreeSkeleton
 
   def branches (tree : InfiniteTreeSkeleton α) : Set (InfiniteList α) := tree.branches_through []
 
-  theorem branches_through_eq_union_children (tree : InfiniteTreeSkeleton α) (node : List Nat) : tree.branches_through node = fun b => ∃ (i : Nat), b ∈ tree.branches_through (i :: node) := by
+  theorem branches_through_eq_union_branches_through_successors (tree : InfiniteTreeSkeleton α) (node : List Nat) : tree.branches_through node = fun b => ∃ (i : Nat), b ∈ tree.branches_through (i :: node) := by
     unfold branches_through
     apply funext
-    simp
+    simp only [List.length_cons, List.reverse_eq_cons_iff, eq_iff_iff]
     intro b
     constructor
     . intro ⟨nodes, h⟩
